#### Лемма
$f(x)\in \mathbb{R}[x]~~~~~c\in\mathbb{C}~~~~~f(c) = 0$ => $f(\overline{c}) = 0$

###### Доказательство
$f = a_nx^n~+~...~+~a_1x~+~a_0~~~~~a_i\in \mathbb{R}, i = 0,...,n$
$f(c) = a_nc^n~+~...~+~a_1c~+~a_0 = 0$
$\overline{f(c)} = \overline{a_nc^n~+~...~+~a_1c~+~a_0} = \overline{a_nc^n}~+~...~+~\overline{a_1c}~+~\overline{a_0} = a_n\overline{c^n}~+~...~+~a_1\overline{c}~+~a_0 = f(\overline{c})$ 
=> $\overline{c}$ - корень

### Теорема (неприводимые многочлены на $\mathbb{R}$)
Неприводимыми многочленами над $\mathbb{R}$ являются:
1) $ax + b$
2) $ax^2 + bx + c,~~~~D<0$

###### Доказательство
$f \in \mathbb{R}[x],~~deg~f>1$
$Над~~\mathbb{C}~~f = a_n\prod_{i = 1}^n (x - c_i),~c_i \in \mathbb{C}$ 
$если~c_j\in \mathbb{C}:~c_j = \alpha + \beta i~-~корень$ 
=> $(по~Лемме)~~~~\overline{c_j} = \alpha - \beta i~-~корень$
=> $в~разложении~есть:~~(x - \alpha - \beta i)(x - \alpha + \beta i) = (x - \alpha)^2 + \beta^2 = x^2 - 2x\alpha + \alpha^2 + \beta^2 \in \mathbb{R}[x]$ 

###### Следствие (каноническое разложение над $\mathbb{R}$)
$f \in \mathbb{R}[x]$ => $f = a\prod_i (x - \gamma_i)^{s_i} \prod_k (x^2 + \alpha_k*x + \beta_k)^{t_k}$ 
$\gamma_i, \alpha_k, \beta_k \in \mathbb{R},~\forall k~~\alpha_k^2 - 4\beta_k < 0,~все~многочлены~различны$

###### Пример:
$x^4 + 1 = x^4 + 2x^2 + 1 - 2x^2 = (x^2 + 1)^2 - (\sqrt{2}x)^2 = (x^2 - \sqrt{2}x + 1)(x^2 + \sqrt{2}x + 1)$
$x^4 + 1 = 0~~~~x^4 = -1~~~~arg(-1) = \pi~~~|-1| = 1$ 
$z_k = \cos\frac{\pi + 2\pi k}{4} + i\sin\frac{\pi + 2\pi k}{4};~~k = 0,1,2,3$ 
$z_0 = \frac{1}{\sqrt{2}} + \frac{1}{\sqrt{2}}i$
$z_1 = -\frac{1}{\sqrt{2}} + \frac{1}{\sqrt{2}}i$
$z_2 = -\frac{1}{\sqrt{2}} - \frac{1}{\sqrt{2}}i$
$z_3 = \frac{1}{\sqrt{2}} - \frac{1}{\sqrt{2}}i$
$x^4 + 1 = (x - \frac{1}{\sqrt{2}} - \frac{1}{\sqrt{2}}i)(x + \frac{1}{\sqrt{2}} - \frac{1}{\sqrt{2}}i)(x - \frac{1}{\sqrt{2}} + \frac{1}{\sqrt{2}}i)(x + \frac{1}{\sqrt{2}} + \frac{1}{\sqrt{2}}i) = ((x - \frac{1}{\sqrt{2}})^2 + \frac{1}{2})((x + \frac{1}{\sqrt{2}})^2 + \frac{1}{2})$ 