### Определение
$f \in K[x],~K~-~поле$
$f = a_nx^n~+~a_{n - 1}x^{n - 1}~+~...~+~a_1x~+~a_0$
**Производной** многочлена $f$ называется многочлен
$f' = na_nx^{n - 1}~+~(n - 1)a_{n - 1}x^{n - 2}~+~...~+~a_1$

###### Свойства
1) $a \in K,~~a' = 0$
2) $a \in K,~~f\in K[x]~~~~(a*f)' = af'$
3) $(f \pm g)' = f' \pm g'$ 
4) $(fg)' = f'g + fg'$
5) $f_i \in K[x],~i=1,...,s~~~~(f_1 * ... * f_s)' = f_1'f_2...f_s + f_1f_2'...f_s + ... + f_1f_2...f_s'$
6) $(f^m)' = mf^{m - 1}f'$ 

###### Доказательство
1)-3) - проверка определения
4) i) $f = a_nx^n,~g = b_mx^m$
	$(a_nx^n*b_mx^m)' = a_nb_m(n + m)x^{n + m - 1}$
	$(a_nx^n)'b_mx^m + a_nx^n(b_mx^m)' = a_nb_mnx^{n - 1 + m} + a_nb_mmx^{n + m - 1}$ => ф-ла 4) верна
	ii) $f = a_nx^n~~g=b_mx^m+...+b_1x + b_0$
	$(fg)' = (a_nx^nb_mx^m~+~...~+~a_nx^nb_1x~+~a_nx^nb_0)' =$$=(a_nx^nb_mx^m)'~+~...~+~(a_nx^nb_0)' = (f)'() + (f)()' = (f)'(~~типо~g~~) + fg'$ 
	iii) $f = a_nx^n~+~...~+~a_1x~+~a_0;~~g = b_mx^m~+~...~+~bx~+~b_0$
	$(fg)' = (a_nx^ng~+~...~+~a_1xg~+~a_0g)' = f'g + fg'$
5) индукция s = 2 - доказано
	$((f_1...f_{s - 1}) f_s)' = (f_1...f_{s - 1})'f_s + (f_1...f_{s - 1})f_s' =~по~предположению~индукции~ +()f_s'$ 
6) $f_1 = f_2 = ... = f_m = f~воспользуемся~5)$
 